Progress on simrel for final graph

src/reordering/ReorderingReexec.v
@@ -8,6 +8,7 @@ Require Import SimrelCommon.
 Require Import StepOps.
 Require Import AuxInj.
 Require Import SubToFullExec.
+Require Import ReorderingFakeSrf.
 
 From hahn Require Import Hahn.
 From hahnExt Require Import HahnExt.
@@ -15,7 +16,242 @@ From imm Require Import Events Execution Execution_eco.
 Require Import Setoid Morphisms Program.Basics.
 Require Import xmm_s_hb.
 
-Module ReorderingReexec.
+Module ReorderingReexecInternal.
+
+Section ReorderingReexecInternal.
+
+Variable X_t X_t' X_s X_s' : WCore.t.
+Variable a_t b_t a_t' b_t' : actid.
+Variable mapper : actid -> actid.
+Variable f : actid -> actid.
+Variable dtrmt cmt : actid -> Prop.
+
+Notation "'R' G" := (fun e => is_true (is_r (lab G) e)) (at level 1).
+Notation "'F' G" := (fun e => is_true (is_f (lab G) e)) (at level 1).
+Notation "'W' G" := (fun e => is_true (is_w (lab G) e)) (at level 1).
+Notation "'Acq' G" := (fun e => is_true (is_acq (lab G) e)) (at level 1).
+Notation "'Rlx' G" := (fun e => is_true (is_rlx (lab G) e)) (at level 1).
+Notation "'Rel' G" := (fun e => is_true (is_rel (lab G) e)) (at level 1).
+
+Notation "'G_t'" := (WCore.G X_t).
+Notation "'G_t''" := (WCore.G X_t').
+Notation "'G_s'" := (WCore.G X_s).
+Notation "'G_s''" := (WCore.G X_s').
+
+Notation "'lab_t'" := (lab G_t).
+Notation "'val_t'" := (val lab_t).
+Notation "'loc_t'" := (loc lab_t).
+Notation "'same_loc_t'" := (same_loc lab_t).
+Notation "'E_t'" := (acts_set G_t).
+Notation "'sb_t'" := (sb G_t).
+Notation "'rf_t'" := (rf G_t).
+Notation "'co_t'" := (co G_t).
+Notation "'rmw_t'" := (rmw G_t).
+Notation "'rpo_t'" := (rpo G_t).
+Notation "'rmw_dep_t'" := (rmw_dep G_t).
+Notation "'data_t'" := (data G_t).
+Notation "'ctrl_t'" := (ctrl G_t).
+Notation "'addr_t'" := (addr G_t).
+Notation "'W_t'" := (fun x => is_true (is_w lab_t x)).
+Notation "'R_t'" := (fun x => is_true (is_r lab_t x)).
+Notation "'Loc_t_' l" := (fun e => loc_t e = l) (at level 1).
+
+Notation "'lab_t''" := (lab G_t').
+Notation "'val_t''" := (val lab_t').
+Notation "'loc_t''" := (loc lab_t').
+Notation "'same_loc_t''" := (same_loc lab_t').
+Notation "'E_t''" := (acts_set G_t').
+Notation "'sb_t''" := (sb G_t').
+Notation "'rf_t''" := (rf G_t').
+Notation "'co_t''" := (co G_t').
+Notation "'rmw_t''" := (rmw G_t').
+Notation "'rpo_t''" := (rpo G_t').
+Notation "'rmw_dep_t''" := (rmw_dep G_t').
+Notation "'data_t''" := (data G_t').
+Notation "'ctrl_t''" := (ctrl G_t').
+Notation "'addr_t''" := (addr G_t').
+Notation "'W_t''" := (fun x => is_true (is_w lab_t' x)).
+Notation "'R_t''" := (fun x => is_true (is_r lab_t' x)).
+Notation "'Loc_t_'' l" := (fun e => loc_t' e = l) (at level 1).
+
+Notation "'lab_s'" := (lab G_s).
+Notation "'val_s'" := (val lab_s).
+Notation "'loc_s'" := (loc lab_s).
+Notation "'same_loc_s'" := (same_loc lab_s).
+Notation "'E_s'" := (acts_set G_s).
+Notation "'loc_s'" := (loc lab_s).
+Notation "'sb_s'" := (sb G_s).
+Notation "'rf_s'" := (rf G_s).
+Notation "'co_s'" := (co G_s).
+Notation "'rmw_s'" := (rmw G_s).
+Notation "'rpo_s'" := (rpo G_s).
+Notation "'rmw_dep_s'" := (rmw_dep G_s).
+Notation "'data_s'" := (data G_s).
+Notation "'ctrl_s'" := (ctrl G_s).
+Notation "'addr_s'" := (addr G_s).
+Notation "'W_s'" := (fun x => is_true (is_w lab_s x)).
+Notation "'R_s'" := (fun x => is_true (is_r lab_s x)).
+Notation "'F_s'" := (F G_s).
+Notation "'vf_s'" := (vf G_s).
+Notation "'srf_s'" := (srf G_s).
+Notation "'Loc_s_' l" := (fun e => loc_s e = l) (at level 1).
+Notation "'Val_s_' l" := (fun e => val_s e = l) (at level 1).
+Notation "'Rlx_s'" := (Rlx G_s).
+Notation "'Acq_s'" := (Acq G_s).
+Notation "'Rel_s'" := (Rel G_s).
+
+Notation "'lab_s''" := (lab G_s').
+Notation "'val_s''" := (val lab_s').
+Notation "'loc_s''" := (loc lab_s').
+Notation "'same_loc_s''" := (same_loc lab_s').
+Notation "'same_val_s''" := (same_val lab_s').
+Notation "'E_s''" := (acts_set G_s').
+Notation "'loc_s''" := (loc lab_s').
+Notation "'sb_s''" := (sb G_s').
+Notation "'rf_s''" := (rf G_s').
+Notation "'co_s''" := (co G_s').
+Notation "'rmw_s''" := (rmw G_s').
+Notation "'rpo_s''" := (rpo G_s').
+Notation "'rmw_dep_s''" := (rmw_dep G_s').
+Notation "'data_s''" := (data G_s').
+Notation "'ctrl_s''" := (ctrl G_s').
+Notation "'addr_s''" := (addr G_s').
+Notation "'W_s''" := (fun x => is_true (is_w lab_s' x)).
+Notation "'R_s''" := (fun x => is_true (is_r lab_s' x)).
+Notation "'F_s''" := (F G_s').
+Notation "'vf_s''" := (vf G_s').
+Notation "'srf_s''" := (srf G_s').
+Notation "'Loc_s_'' l" := (fun e => loc_s' e = l) (at level 1).
+Notation "'Val_s_'' l" := (fun e => val_s' e = l) (at level 1).
+Notation "'Rlx_s''" := (Rlx G_s').
+Notation "'Acq_s''" := (Acq G_s').
+Notation "'Rel_s''" := (Rel G_s').
+
+Notation "'Tid_' t" := (fun e => tid e = t) (at level 1).
+
+(* Id aliases for better readability *)
+Definition a_s := b_t.
+Definition b_s := a_t.
+Definition a_s' := b_t'.
+Definition b_s' := a_t'.
+Definition A_s' := extra_a X_t' a_t' b_t' a_s'.
+
+Definition mapper' := upd (upd id a_t' a_s') b_t' b_s'.
+Definition G_s'' : execution := {|
+  acts_set := mapper' ↑₁ E_t';
+  threads_set := threads_set G_t';
+  lab := lab_t' ∘ mapper';
+  rf := mapper' ↑ rf_t';
+  co := mapper' ↑ co_t';
+  rmw := mapper' ↑ rmw_t';
+  rmw_dep := rmw_dep_s;
+  ctrl := ctrl_s;
+  data := data_s;
+  addr := addr_s;
+|}.
+
+Record reexec_conds : Prop := {
+  rc_a_dtrmt : dtrmt a_t <-> dtrmt a_t';
+  rc_b_dtrmt : dtrmt b_t <-> dtrmt b_t';
+  rc_a_eq : dtrmt a_t -> a_t = a_t';
+  rc_b_eq : dtrmt b_t -> b_t = b_t';
+  rc_pres : b_t = b_t' -> a_t = a_t';
+  rc_simrel : reord_simrel X_s X_t a_t b_t mapper;
+  rc_step : WCore.reexec X_t X_t' f dtrmt cmt;
+  rc_inv_start : reord_step_pred X_t a_t b_t;
+  rc_inv_end : reord_step_pred X_t' a_t' b_t';
+  rc_l_a_nacq : Rlx_s' a_s';
+  rc_vf : forall (IMB : E_t' b_t') (NINA : ~ E_t' a_t'),
+            vf_s' ⨾ sb_s' ⨾ ⦗eq a_s'⦘ ≡ vf G_s'' ⨾ sb_s' ⨾ ⦗eq a_s'⦘;
+  (**)
+  rc_extra_lab : fake_srf G_s'' a_s' (lab_s' a_s') ⨾ ⦗A_s' ∩₁ WCore.lab_is_r (lab_s' a_s')⦘ ⊆ same_val_s';
+  rc_lab : eq_dom E_t' (lab_s' ∘ mapper') lab_t';
+  rc_acts : E_s' ≡₁ mapper' ↑₁ E_t' ∪₁ extra_a X_t' a_t' b_t' a_s';
+  rc_rf : rf_s' ≡ mapper' ↑ rf_t' ∪ fake_srf G_s'' a_s' (lab_s' a_s') ⨾ ⦗A_s' ∩₁ WCore.lab_is_r (lab_s' a_s')⦘;
+  rc_co : co_s' ≡ mapper' ↑ co_t' ∪
+          add_max
+            (extra_co_D (mapper' ↑₁ E_t') lab_s (WCore.lab_loc (lab_s' a_s')))
+            (A_s' ∩₁ WCore.lab_is_w (lab_s' a_s'));
+  rc_rmw : rmw_s ≡ mapper ↑ rmw_t;
+  rc_threads : threads_set G_s ≡₁ threads_set G_t;
+  rc_ctrl : ctrl_s' ≡ ctrl_s;
+  rc_data : data_s' ≡ data_s;
+  rc_addr : addr_s' ≡ addr_s;
+  rc_rmw_dep : rmw_dep_s' ≡ rmw_dep_s;
+}.
+
+Lemma mapinj : inj_dom E_t' mapper'.
+Proof using.
+  admit.
+Admitted.
+
+Lemma intermediate_graph_wf
+    (INB : E_t' b_t')
+    (NINA : ~ E_t' a_t')
+    (CTX : reexec_conds) :
+  Wf G_s''.
+Proof using.
+  admit. (* This graph is very conveniently mapped by m *)
+Admitted.
+
+Lemma reexec_simrel
+    (CTX : reexec_conds) :
+  reord_simrel X_s' X_t' a_t' b_t' mapper'.
+Proof using.
+  assert (EXAR : eq b_t' ∩₁ R_s' ≡₁ eq b_t' ∩₁ WCore.lab_is_r (lab_s' a_s')).
+  { unfold a_s', is_r, WCore.lab_is_r.
+    unfolder; split; ins; desf. }
+  assert (SRF :
+    fake_srf G_s'' a_s' (lab_s' a_s') ⨾ ⦗A_s' ∩₁ WCore.lab_is_r (lab_s' a_s')⦘ ≡
+    srf_s' ⨾ ⦗extra_a X_t' a_t' b_t' b_t' ∩₁ R_s'⦘
+  ).
+  { unfold A_s', extra_a; desf; [desf | basic_solver 11].
+    rewrite EXAR, <- fake_srf_is_srf with (G_s := G_s'').
+    all: ins.
+    { apply intermediate_graph_wf; auto. }
+    { unfold fake_sb, G_s'', sb. ins.
+      rewrite (rc_acts CTX), extra_a_some; auto. }
+    { unfold G_s'', mapper'. ins. intro FALSO.
+      admit. (* Invert the mapper *) }
+    { unfold G_s''. ins.
+      admit. (* TODO *) }
+    { apply CTX; auto. }
+    rewrite (rc_co CTX), seq_union_l.
+    unfold A_s'. rewrite extra_a_some; auto.
+    admit. (* TODO: add_max_eq_r *) }
+  constructor; ins.
+  { apply mapinj. }
+  { unfolder. unfold extra_a; ins; desf.
+    constructor; [red; auto | desf].
+    rewrite extra_a_some in SRF; auto.
+    rewrite <- SRF. apply CTX. }
+  { rewrite (rc_acts CTX), set_minus_union_l.
+    unfold a_s'. rewrite set_minusK, set_union_empty_r.
+    unfold extra_a; desf; [| clear; basic_solver].
+    rewrite set_minus_disjoint; auto with hahn.
+    admit. (* a_t' is not in *) }
+  { admit. (* TODO *) }
+  { admit. (* TODO *) }
+  { apply CTX. }
+  { apply CTX. }
+  { admit. }
+  { rewrite <- SRF, (rc_rf CTX). auto. }
+  { rewrite (rc_co CTX). admit. }
+  { admit. }
+  { admit. }
+  { admit. }
+  { admit. }
+  { admit. }
+  { admit. }
+  { admit. (* rpo *) }
+  { admit. }
+  { admit. }
+  admit.
+Admitted.
+
+End ReorderingReexecInternal.
+
+End ReorderingReexecInternal.
 
 Section ReorderingReexec.
 
@@ -134,110 +370,13 @@ Proof using CTX.
   admit.
 Admitted.
 
-Lemma mapinj : inj_dom E_t' mapper'.
-Proof using CTX.
-  admit.
-Admitted.
-
 Definition cmt' := mapper' ↑₁ (cmt ∪₁ extra_b).
 Definition dtrmt' := mapper' ↑₁ (dtrmt \₁ extra_b).
 Definition f' := mapper' ∘ f ∘ mapper'.
 (* Intermediate graph for locating the srf edge for for a_s *)
-Definition G_s'' : execution := {|
-  acts_set := mapper' ↑₁ E_t';
-  threads_set := threads_set G_t';
-  lab := lab_t' ∘ mapper';
-  rf := mapper' ↑ rf_t';
-  co := mapper' ↑ co_t';
-  rmw := mapper' ↑ rmw_t';
-  rmw_dep := rmw_dep_s;
-  ctrl := ctrl_s;
-  data := data_s;
-  addr := addr_s;
-|}.
-
-Lemma intermediate_graph_wf
-    (INB : E_t' b_t')
-    (NINA : ~ E_t' a_t') :
-  Wf G_s''.
-Proof using CTX.
-  admit. (* This graph is very conveniently mapped by m *)
-Admitted.
-
-Lemma intermediate_graph_cons
-    (INB : E_t' b_t')
-    (NINA : ~ E_t' a_t') :
-  irreflexive (hb G_s'' ⨾ (eco G_s'')^?).
-Proof using CTX.
-  admit. (* True by monotonicity *)
-Admitted.
 
 Definition A_s' := extra_a X_t' a_t' b_t' a_s'.
 Definition E_s' := mapper' ↑₁ E_t' ∪₁ A_s'.
-Definition sb_s' := ⦗E_s'⦘ ⨾ ext_sb ⨾ ⦗E_s'⦘.
-
-(* 'fake' srf. we later show that it is equal to srf ; [a_s'] *)
-Definition srf_s'' :=
-  (
-    vf_s ⨾ sb_s' ⨾ ⦗A_s'⦘ ∩
-    (fun x _ => loc_s x = WCore.lab_loc l_a')
-  ) ⨾ ⦗WCore.lab_is_r l_a'⦘
-    \ (co_s ⨾ vf_s ⨾ sb_s' ⨾ ⦗A_s'⦘).
-
-(* Some fake srf props *)
-
-(* The 'final' graph *)
-Definition G_s' : execution := {|
-  acts_set := mapper' ↑₁ E_t' ∪₁ A_s';
-  threads_set := threads_set G_t';
-  lab := lab_t' ∘ mapper';
-    rf := mapper' ↑ rf_t' ∪
-          srf_s'';
-    co := mapper' ↑ co_t' ∪
-          add_max
-            (extra_co_D (mapper' ↑₁ E_t') lab_s (WCore.lab_loc l_a'))
-            (A_s' ∩₁ WCore.lab_is_w l_a');
-  rmw := mapper' ↑ rmw_t';
-  rmw_dep := rmw_dep_s;
-  ctrl := ctrl_s;
-  data := data_s;
-  addr := addr_s;
-|}.
-Definition X_s' := {|
-  WCore.sc := WCore.sc X_s;
-  WCore.G := G_s';
-|}.
-
-Lemma final_graph_with_srf_wf
-    (INB : E_t' b_t')
-    (NINA : ~ E_t' a_t') :
-  Wf G_s''.
-Proof using CTX.
-  admit. (* We added an edge and a_s to intermediate graph *)
-Admitted.
-
-Lemma final_graph_with_srf_cons
-    (INB : E_t' b_t')
-    (NINA : ~ E_t' a_t') :
-  irreflexive (hb G_s'' ⨾ (eco G_s'')^?).
-Proof using CTX.
-  admit. (* TODO (ask Evgenii) *)
-Admitted.
-
-(* Srf goodness *)
-Lemma final_graph_with_srf_srf :
-  (rf G_s'') ⨾ ⦗A_s'⦘ ≡ (srf G_s'') ⨾ ⦗A_s'⦘.
-Proof using CTX.
-  admit.
-Admitted.
-
-Lemma final_graph_simrel :
-  reord_simrel X_s' X_t' a_t' b_t' mapper'.
-Proof using CTX.
-  constructor; ins.
-  { apply mapinj. }
-  { admit. }
-Admitted.
 
 Lemma simrel_reexec :
   exists mapper' X_s' f' dtrmt' cmt',
@@ -245,8 +384,6 @@ Lemma simrel_reexec :
     << STEP : WCore.reexec X_s X_s' f' dtrmt' cmt' >>.
 Proof using CTX.
 Admitted.
-
-End ReorderingReexec.
 
 End ReorderingReexec.
 
